

Show that $m(a+bx) = a + b \times m(x)$ (Part 1)

$$m(y) = \frac{1}{N} \sum_{i=1}^N y_i \quad \text{and} \quad y_i = a + bx_i$$

Using this logic ...

$$m(a+bx) = \frac{1}{N} \sum_{i=1}^N (a + bx_i)$$

$$m(a+bx) = \frac{1}{N} \sum_{i=1}^N a + bx_i = \frac{a}{N} \sum_{i=1}^N 1 + \frac{b}{N} \sum_{i=1}^N x_i = a + \frac{b}{N} \sum_{i=1}^N x_i$$

$$a + b \left(\frac{1}{N} \sum_{i=1}^N x_i \right) = m(x)$$

$$\therefore a + b \times m(x) = m(a+bx) \quad \checkmark \text{ linear}$$

Show that $\text{cov}(x, x) = s^2$ (Part 2)

$$\text{cov}(x, x) = \frac{1}{N} \sum_{i=1}^N (x_i - m(x))(x_i - m(x))$$

$$= \frac{1}{N} \sum_{i=1}^N (x_i - m(x))^2 = s^2$$

$$\therefore \text{cov}(x, x) = s^2 \quad \checkmark$$

Show that $\text{cov}(x, a+by) = b \text{cov}(x, y)$ (Part 3)

$$\text{cov}(x, a+by) = \frac{1}{N} \sum_{i=1}^N (x_i - m(x))[(a + by_i) - (a + b m(y))]$$

$$= \frac{1}{N} \sum_{i=1}^N (x_i - m(x)) b (y_i - m(y))$$

$$= b \left(\frac{1}{N} \sum_{i=1}^N (x_i - m(x))(y_i - m(y)) \right) \quad \text{* given function}$$

$$\text{cov}(x, a+by) = b \text{cov}(x, y) \quad \checkmark$$

Show that $\text{cov}(a+bx, a+by) = b^2 \text{cov}(x, y)$ (part 4)

$$\begin{aligned}\text{cov}(a+bx, a+by) &= \frac{1}{n} \sum_{i=1}^n [(a+bx_i) - (a+b\bar{x})][(a+by_i) - (a+b\bar{y})] \\&= \frac{1}{n} \sum_{i=1}^n b(x_i - \bar{x}) b(y_i - \bar{y}) \\&= b^2 \left(\frac{1}{n} \sum_{i=1}^n (x_i - \bar{x})(y_i - \bar{y}) \right)\end{aligned}$$

Given

$\text{cov}(a+bx, a+by) = b^2 \text{cov}(x, y) \quad \checkmark$

Part 5

For $b > 0$, the data is only increasing and order is preserved. This means that for the median value of x , the median value of $a+bx$ will be equal to the median value of $a+b\text{med}(x)$.

So yes, $\text{med}(a+bx) = a + b\text{med}(x) \quad \checkmark$

Proof: $x = \{2, 4, 6, 8, 10\}$ where $a = 2, b = 2$

$$a+bx = \{6, 10, 14, 18, 22\}$$

$$\text{med}(a+bx) = 14$$

$$a+b\text{med}(x) = 2 + 2(6) = 14$$

} Values match \checkmark

for IQR: $\text{IQR} = Q_{.75} - Q_{.25} \xrightarrow{\text{linear transformation}} (a+bQ_{.75}) - (a+bQ_{.25}) = b(Q_{.75} - Q_{.25})$

$$\therefore \text{IQR}(a+bx) = b \cdot \text{IQR}(x)$$

$\therefore \text{IQR}(a+bx) \neq a + b\text{IQR}(x)$ as a is canceled

Part 6

Example: $x = \{2, 4, 6, 8, 10\}$

$$m(x) = \frac{2+4+6+8+10}{5} = 6 \rightarrow (m(x))^2 = 36$$

$$\text{and } \sqrt{m(x)} = \sqrt{6} = 2.45$$

$$x^2 = \{4, 16, 36, 64, 100\}$$

$$m(x^2) = \frac{4+16+36+64+100}{5} = 44$$

$$44 \neq 36$$
$$m(x^2) \neq (m(x))^2$$

$$\sqrt{x} = \{\sqrt{2}, 2, \sqrt{6}, 2\sqrt{2}, \sqrt{10}\}$$

$$m(\sqrt{x}) = \frac{\sqrt{2} + 2 + \sqrt{6} + 2\sqrt{2} + \sqrt{10}}{5} = 2.37$$

$$2.37 \neq 2.45$$

$$m(\sqrt{x}) \neq \sqrt{m(x)}$$